Readd quote but at all types this time.
This is just the reduction part, no typing yet.

theories/AutoSubst/Ast.sig
@@ -24,6 +24,7 @@ tId : term -> term -> term -> term
 tRefl : term -> term -> term
 tIdElim : term -> term -> (bind term , term in term) -> term -> term -> term -> term
 
+tQuote : term -> term -> term
 tDecide : term -> term -> term -> term
 tReflect : term -> term -> term -> term -> term
 tReify : term -> term -> term -> term -> term
