theories/Syntax/Closed.v
@@ -33,6 +33,7 @@ match t with
   (andb (is_closedn n x)
   (andb (is_closedn (S (S n)) P)
     (andb (is_closedn n hr) (andb (is_closedn n y) (is_closedn n e)))))
+| tQuote A t => andb (is_closedn n A) (is_closedn n t)
 | tDecide A t u =>
   andb (is_closedn n A)
     (andb (is_closedn n t) (is_closedn n u))
